
\section*{Proof By Induction}

\begin{itemize}
\item \textbf{Base Step}
\item \textbf{Induction Step}
\item \textbf{Some Step}
\end{itemize}

%------------------------- %
%-------------------------- %



\section{Proof By Induction}

Prove by Induction the following expression
\[ \sum_{r=1}^{r=n} r^2 = \frac{n(n+1)(2n+1)}{6} \]
for all $n \in N_0$.


\begin{itemize}
	\item \textbf{Step 1} : Is the proposition true for $n = 1$?
	\item \textbf{Step 2} : Show that if the proposition is true for $n=k$, then it is also true for $n=k+1$.
	\item \textbf{Step 3} : Conclude that the proposition is true for all natural numbers greater than or equal to one.
\end{itemize}

%------------------------------------------------ %

\subsection{Proof By Induction}

Prove by induction the following expression
\[ \sum_{r=1}^{r=n} r^2 = \frac{n(n+1)(2n+1)}{6} \]
for all $n \in N_0$.
\begin{itemize}
	\item \textbf{Step 1} : Is the proposition true for $n = 1$? 
\end{itemize}
\textbf{Left-hand side}
\[ \sum_{r=1}^{r=1} r^2 = 1^2 = 1 \]



\textbf{Left-hand side}
\[ \sum_{r=1}^{r=1} r^2 = 1^2 = \boldsymbol{1} \]
\textbf{Right-hand side}

\[ \frac{n(n+1)(2n+1)}{6}  = \frac{1(1+1)(2\cdot 1+1)}{6} \]
\[  = \frac{1\times 2 \times 3}{6} = \frac{6}{6}=\boldsymbol{1} \]

%------------------------------------------------ %


\begin{itemize}
	\item \textbf{Step 1} : Is the proposition true for $n = 1$? 
\end{itemize}
\bigskip
Yes: The left-hand side and right-hand side of the equation yield the same value.

\begin{itemize}
	\item \textbf{Step 2} : Show that if the proposition is true for $n=k$, then it is also true for $n=k+1$.
\end{itemize}
Given: \[ \sum_{r=1}^{r=k} r^2 = \frac{k(k+1)(2k+1)}{6} \]

To Prove: \[ \sum_{r=1}^{r=k+1} r^2 = \frac{(k+1)(k+2)(2k+3)}{6} \]


%------------------------------------------------ %

\subsection{Proof By Induction}
%% - \vspace{-1cm}



\[ \sum_{r=1}^{r=k+1} r^2 = 1^2 + 2^2 + 3^2 + \ldots + k^2 + (k+1)^2 \]






\[ \sum_{r=1}^{r=k+1} r^2 = 1^2 + 2^2 + 3^2 + \ldots + k^2 + (k+1)^2 \]

\[ \sum_{r=1}^{r=k+1} r^2 = \boldsymbol{\sum_{r=1}^{r=k} r^2} + (k+1)^2 \]



\[ \sum_{r=1}^{r=k+1} r^2 = \boldsymbol{\sum_{r=1}^{r=k} r^2} + (k+1)^2 \]

\[ \sum_{r=1}^{r=k+1} r^2 = \frac{k(k+1(2k+1
	))}{6} + (k+1)^2 \]

