%\documentclass[11pt, a4paper,dalthesis]{report}    % final 
%\documentclass[11pt,a4paper,dalthesis]{report}
%\documentclass[11pt,a4paper,dalthesis]{book}

\documentclass[11pt,a4paper,titlepage,oneside,openany]{article}

\pagestyle{plain}
%\renewcommand{\baselinestretch}{1.7}

\usepackage{setspace}
%\singlespacing
\onehalfspacing
%\doublespacing
%\setstretch{1.1}

\usepackage{amsmath}
\usepackage{amssymb}
\usepackage{amsthm}

\usepackage[margin=3cm]{geometry}
\usepackage{graphicx,psfrag}%\usepackage{hyperref}


\usepackage{framed}
\include{zcust_preamble}
\include{zcust_commands}

\begin{document}


\pagebreak
\subsection*{Geometric Series}
A \emph{geometric sequence} $a_n=a_0 r^n$ is a sequence whose terms are multiplied constant ratio $r$ at each step. A \emph{geometric series} $s_n$ is the sum of a geometric sequence.
\begin{equation*}
  s_n=\sum_{k=0}^n a_0 r^n =  a_0 \sum_{k=0}^n r^n = a_0 + a_0r +a_0 r^2+a_0 r^3 + \cdots 
\end{equation*}
\noindent \textbf{Example:} Let $a_n=\left(\frac{1}{2}\right)^n$.
\begin{center}
\begin{tabular}{c|c|c|c|c|c|c}
$n$ & $0$ & $1$ & $2$ & $3$ & $4$ & $5$   \\ \hline
$a_n$ & $1$ & $\frac{1}{2}$ & $\frac{1}{4}$ & $\frac{1}{8}$ & $\frac{1}{16}$ & $\frac{1}{32}$  \\ \hline
$s_n$ & $1$ & $1.5$ & $1.75$ & $1.875$ & $1.9375$ & $1.96875$ 
\end{tabular}
\end{center}
As with arithmetic series, instead of having to sum up every term in a geometric series, a formula for the $n^{th}$ term in the series can be derived.
\begin{thm*}
  For a geometric series
  \begin{equation*}
    s_n = a_0 \sum_{k=0}^n r^n= a_0 \left( \frac{1-r^{n+1}}{1-r} \right)
  \end{equation*}
\begin{proof}
To prove this, we need a formula for the sum $S_n=\sum_{k=0}^n r^k$. We proceed proceed by writing out the sum in full, then the sum multiplied by $r$. These two sums are subtracted, resulting in most terms cancelling out.
  \begin{align*}
    S_n&=1+r+r^2+r^3+\cdots+r^{n-1}+r^n\\
    r S_n&=r+r^2+r^3+r^4+\cdots+r+r^{n+1}\\
    S_n-r S_n&= 1 + (r - r) + (r^2-^2)+\cdots+(r^n-r^n)-r^{n+1}
  \end{align*}
The bracketed terms cancel and so
\begin{equation*}
  S_n(1-r)=1 -r^{n+1}, \qquad \Rightarrow S_n=\frac{1-r^{n+1}}{1-r}
\end{equation*}
Multiplying by $a_0$ now gives the required result.
\end{proof}
\end{thm*}
\noindent  \textbf{Example:}
For $a_n=\left(\frac{1}{2}\right)^n$, the formula gives
\begin{equation*}
  s_5=(1)\frac{1-\frac{1}{2^{5+1}}}{1-\frac{1}{2}}=\frac{1-\frac{1}{64}}{\frac{1}{2}}=2\frac{63}{64}=1.96875
\end{equation*}
Which matches what was calculated for $s_5$ in the table above. Further terms can be calculated without summation. For example
\begin{equation*}
  s_{50}=(1)\frac{1-\frac{1}{2^{50+1}}}{1-\frac{1}{2}}=\frac{1-\frac{1}{2^{51}}}{\frac{1}{2}} \cong=1.99999999999999911182
\end{equation*}


\subsection*{Exponential Function}

Since $y=e^x$ can be evaluated for any real $x$, a graph of the function can be drawn. The series \eqref{eq:exp_def_taylor} immediately gives $e^0=1$, and so the graph passes through the point $(0,1)$. $e^1=e \cong 2.781828$ and so the graph passes through $(1,2.781828)$. Other points on the graph are calculated in a similar fashion.

\begin{wrapfigure}{l}{0.4\textwidth}
%  \begin{center} 
   % \includegraphics[width=1.1\textwidth]{exp}
    \includegraphics[width=0.4\textwidth]{images/exp.eps}
%  \end{center}
\end{wrapfigure}
The exponential function grows extremely rapidly as $x \to \infty$. For example, $e^{10}\cong 22,026$ and $e^{100}\cong 2.688 \times 10^{43}$. In fact the function grows faster than any polynomial function, no matter how large the constants or powers. For example for $x\ge50$, $e^x> 53000 x^{10}$. Never use the term \emph{grows exponentially} unless the growth is actually this fast.

Correspondingly the exponential function decreases extremely rapidly as $x \to -\infty$. For example $e^{-10} \cong 0.0000454$ and $e^{-100}\cong 3.72 \times 10^{-44}$. If the height of the graph above the x-axis at $x=0$ was $1$ metre, then the distance between the graph and the axis at $x=-30$ would be less than the radius of an atom. It can be seen that $\lim_{x\to -\infty} e^{x} = 0$. However, note that the function never actually reaches $0$.

The exponential function $e^x$ behaves as the number $e \cong 2.781828$ being put to the power of $x$, and the usual rules for powers apply. For example

\begin{equation*}
  e^{x} e^{y} = e^{x+y} , \qquad e^0=1, \qquad e^x > 0 \text{ for all real } x 
\end{equation*}

One important property of the exponential functions is that the function is its own derivative, that is
\begin{equation*}
  y=e^x, \quad \Rightarrow \frac{dy}{dx}=e^x
\end{equation*}
The derivative is a measure of the rate of growth of the function. Therefore, the rate of growth of $e^x$ is equal to its current value. So the larger the function is, the faster it is growing, and so the rate of growth itself grows and the function quickly becomes enormous. \begin{wrapfigure}{r}{0.4\textwidth}
%  \begin{center} 
   % \includegraphics[width=1.1\textwidth]{exp}
    \includegraphics[width=0.4\textwidth]{images/expd.eps}
%  \end{center}
\end{wrapfigure}Examples of such exponential growth are populations of bacteria, or the growth of bank savings accounts or unpaid loans. In reality, exponential growth cannot continue forever; something eventually has to give, e.g. the bacteria run out of food, or the banking system collapses.

Closely related to the exponential function is the exponential decay function $e^{-x}$. Substituting $-x$ for $x$ in the infinite series for $e^x$ gives
\begin{equation*}
  e^{-x} = \sum_{n=0}^{\infty} \frac{(-1)^n x^n}{n!}=1-x+\frac{x^2}{2!}-\frac{x^3}{3!}+\cdots
\end{equation*}
The graph of this function is the mirror images of $e^x$ in the y-axis. The exponential decay function decreases towards $0$ as $x \to \infty$ and increases infinitely as $x \to -\infty$.

Infinite series can be used to define many kinds of functions.
\subsection*{Trignometric functions}
Trignometric functions such as sine and cosine can be evaluated using infinite series. These functions can be defined by
\begin{align*}
  \cos(x) &= \sum_{n=0}^{\infty} \frac{(-1)^n x^{2n}}{(2n)!}=1-\frac{x^2}{2!}+\frac{x^4}{4!}-\frac{x^6}{6!}+\frac{x^8}{8!}-\cdots\\
  \sin(x) &= \sum_{n=0}^{\infty} \frac{(-1)^n x^{2n+1}}{(2n+1)!}=x-\frac{x^3}{3!}+\frac{x^5}{5!}-\frac{x^7}{7!}+\frac{x^9}{9!}-\cdots
\end{align*}
Using the ratio test, these series can be shown to be convergent for all $x$. For example for $\cos(x)$, the terms are $a_{n}=\dfrac{(-1)^n x^{2n}}{(2n)!}$ and $a_{n+1}=\dfrac{(-1)^{n+1} x^{2n+2}}{(2n+2)!}$ and so
\begin{align*}
  \left| \frac{a_{n+1}}{a_n}\right|&=\left| \frac{(-1)^{n+1} x^{2n+2}}{(2n+2)!} \frac{(2n)!}{(-1)^n x^{2n}}\right|=\left|\frac{(-1)^{n+1}}{(-1)^{n}}\frac{x^{2n+2}}{x^{2n}}\frac{(2n)!}{(2n+2)!}\right|\\
  &=\left|(-1) x^2 \frac{1}{(2n+1)(2n+2)}\right|= \frac{x^2}{4n^2+6n+2}
\end{align*}
\begin{equation*}
  R=\lim_{n \to \infty}   \left| \frac{a_{n+1}}{a_n}\right| = \lim_{n \to \infty} \frac{x^2}{4n^2+6n+2} = 0, \quad \text{ so } R<1 \text{ and so series is cgt.}
\end{equation*}

It is \emph{vital} to note that the angle $x$ used in these infinite series but be measured in radians. If an angle $\theta$ is given in degrees $d$, then the angle can be converted between degress and radians using the following formulas
\begin{equation*}
  x_{\text{radians}} = d^{\circ} \times \frac{\pi}{180}, \qquad d^{\circ} = x_{\text{radians}} \times \frac{180}{\pi}
\end{equation*}

The infinite series can be used to evaluate the cosine of angles by summing the series until a specified accuracy is reached. For example, to calculate the cosine of $60^\circ$, first convert the angle to radians. So the angle in radians is given by $x= 60 \frac{\pi}{180}=\frac{\pi}{3}\cong1.0471798$. Using the series, cosine is given by

\begin{equation*}
  \cos(\frac{\pi}{3}) = \sum_{n=0}^{\infty} \frac{(-1)^n (\frac{\pi}{3})^{2n}}{(2n)!}=1-\frac{\left( \frac{\pi}{3} \right)^2}{2!}+\frac{\left( \frac{\pi}{3} \right)^4}{4!}-\frac{\left( \frac{\pi}{3} \right)^6}{6!}+\frac{\left( \frac{\pi}{3} \right)^8}{8!}-\cdots
\end{equation*}
And can be summed using a table similar to the following. Because the series now ossillates around the limit, instead of waiting for the digits to ``lock-in'' instead evaluate the series until the $a_n$ terms approach zero.
\\

%\begin{tabular}{|l|c|c:c:c:c:c:c:c:c:c:c|c|c:c:c:c:c:c:c:c:c:c|}\hline
\begin{tabular}{|l|c|cp{0.1em}p{0.1em}p{0.1em}p{0.1em}p{0.1em}p{0.1em}p{0.1em}p{0.1em}p{0.1em}|c|p{0.1em}p{0.1em}p{0.1em}p{0.1em}p{0.1em}p{0.1em}p{0.1em}p{0.1em}p{0.1em}p{0.1em}|}\hline
$n$ & \ & \multicolumn{10}{c|}{$a_n$} & \ & \multicolumn{10}{c|}{$s_n$} \\\hline
$0$ & \ &
\hspace{0.4em} & $1$ & $\cdot$ & $0$ & $0$ & $0$ & $0$ & $0$ & $0$ & $0$  & \ &
\hspace{0.4em} & $1$ & $\cdot$ & $0$ & $0$ & $0$ & $0$ & $0$ & $0$ & $0$  \\ \hline
$1$ & \ &
- & $0$ & $\cdot$ & $5$ & $4$ & $8$ & $3$ & $1$ & $1$ & $3$  & \ &
\hspace{0.4em} & $0$ & $\cdot$ & $4$ & $5$ & $1$ & $6$ & $8$ & $8$ & $6$  \\ \hline
$2$ & \ &
\hspace{0.4em} & $0$ & $\cdot$ & $0$ & $5$ & $0$ & $1$ & $0$ & $7$ & $5$  & \ &
\hspace{0.4em} & $0$ & $\cdot$ & $5$ & $0$ & $1$ & $7$ & $9$ & $6$ & $2$  \\ \hline
$3$ & \ &
- & $0$ & $\cdot$ & $0$ & $0$ & $1$ & $8$ & $3$ & $1$ & $6$  & \ &
\hspace{0.4em} & $0$ & $\cdot$ & $4$ & $9$ & $9$ & $9$ & $6$ & $4$ & $5$  \\ \hline
$4$ & \ &
\hspace{0.4em} & $0$ & $\cdot$ & $0$ & $0$ & $0$ & $0$ & $3$ & $5$ & $8$  & \ &
\hspace{0.4em} & $0$ & $\cdot$ & $5$ & $0$ & $0$ & $0$ & $0$ & $0$ & $4$  \\ \hline
$5$ & \ &
- & $0$ & $\cdot$ & $0$ & $0$ & $0$ & $0$ & $0$ & $0$ & $0$  & \ &
\hspace{0.4em} & $0$ & $\cdot$ & $4$ & $9$ & $9$ & $9$ & $9$ & $9$ & $9$  \\ \hline
$5$ & \ &
\hspace{0.4em} & $0$ & $\cdot$ & $0$ & $0$ & $0$ & $0$ & $0$ & $0$ & $0$  & \ &
\hspace{0.4em} & $0$ & $\cdot$ & $5$ & $0$ & $0$ & $0$ & $0$ & $0$ & $0$  \\ \hline
\end{tabular}
\\
\\
And so $\cos(\frac{\pi}{3}) \cong 0.5$. In fact, the cosine of $60^\circ$ is exactly $\frac{1}{2}$.

In this way, the cosine and sine functions can be evaluated for all $x$ and the functions can be graphed as shown below. Note that the angles are measured in radians.
\begin{figure}[b]
  \begin{center}
    \includegraphics[width=0.9\textwidth]{images/cos_sin.eps}
  \end{center}
\end{figure}
\pagebreak

\subsection*{Logarithim function}

The natural logarithim $\log(x)=\log_{e}(x)=\ln(x)$ can be defined using the infinite series
\begin{equation*}
  \log(1+x) = \sum_{n=1}^{\infty} \frac{(-1)^{n+1} x^n}{n}=x-\frac{x^2}{2}+\frac{x^3}{3}-\frac{x^4}{4}+ \cdots 
\end{equation*}

\begin{wrapfigure}{l}{0.4\textwidth}
%  \begin{center} 
   % \includegraphics[width=1.1\textwidth]{exp}
    \includegraphics[width=0.4\textwidth]{images/log.eps}
%  \end{center}
\end{wrapfigure}
However, when the ratio test is applied, the convergence of $\log$ depends on the value of $x$
\begin{align*}
  \left| \frac{a_{n+1}}{a_n}\right|&=\left| \frac{(-1)^{n+2} x^{n+1}}{n+1} \frac{n}{(-1)^{n+1} x^n}\right|\\
&=|x|\left(\frac{n+1}{n}\right)\\
 \Rightarrow R &=\lim_{n \to \infty} |x|\left(\frac{n+1}{n}\right) = x
\end{align*}
And so $R=|x|$, and hence the series will be convergent only when $|x|<1$. And when $|x|>1$ the series is divergent. So only values of $\log$ in the interval $(0,2)$ can be computed using this infinite series.

A better method of calculating $\log$ is needed. One method is to remember the definition of the $\log$ function. The number $x=\log(D)$ is the $x$ which satisfies $e^X=D$. This can be rewritten as $e^x-D=0$. Consider the function
\begin{equation*}
  f(x)=e^x-D
\end{equation*}
If an $x$ can be found which gives $f(x)=0$, then $x=\log(D)$. This is the problem of finding the root of the function, and one way to solve this problem is to use Newton's Method.


% 0.000000000000000   1.000000000000000   1.000000000000000
%   1.000000000000000  -0.548311355616075   0.451688644383925
%   2.000000000000000   0.050107557116256   0.501796201500181
%   3.000000000000000  -0.001831636171268   0.499964565328913
%   4.000000000000000   0.000035868104002   0.500000433432915
%   5.000000000000000  -0.000000437041972   0.499999996390943

% \thispagestyle{empty} 
% \begin{landscape}
% \begin{figure}[!h!]
%  \begin{centering}
%    \includegraphics[width=1.7\textwidth]{cosine}
%    \includegraphics[width=1.7\textwidth]{sine}
%  \end{centering}
% \end{figure}
% \end{landscape}

% \pagebreak
% \thispagestyle{empty} 
%   \begin{figure}[!h!]
%     \begin{center}
%       %\includegraphics[width=1.1\textwidth]{exp}
%       \includegraphics[scale=1.85]{exp}
%     \end{center}
%   \end{figure}
% \pagebreak
% \thispagestyle{empty} 
%   \begin{figure}[!h!]
%     \begin{center}
%     %\includegraphics[width=1.1\textwidth]{log}
%       \includegraphics[scale=1.85]{log}
%     \end{center}
%   \end{figure}
% \pagebreak
% \thispagestyle{empty} 
%   \begin{figure}[!h!]
%     \begin{center}
%     \includegraphics[width=0.55\textwidth]{exp2}
%     \end{center}
%   \end{figure}



\end{document}

